# Math

## Simpler quadratic formula

First rearrange to get form in which leading coefficient for the xÂ² term
is 1, and only one constant.

$$ x^2 + Bx + C = 0 $$

Factor generally

$$ x^2 + Bx + C = 0 = (x - R)(x - S) $$

$$ (x - R)(x - S) = x^2 - (R + S)x + RS $$

$$ -B = (R + S) $$

Divide both sides by 2

$$ \frac{-B}{2} = \frac{R+S}{2}  $$

So $-B/2$ is the average of the two values we were looking for.

So R and S are values like:

$$ -B / 2 + z $$

$$ -B / 2 - z $$

Multiplying the two together is equal to $C$.

$$ \left( \frac{B}{2} \right)^2 - z^2 = C $$

$$ z = \sqrt{ \left( \frac{B}{2} \right)^2  - C } $$

The final solutions are then

$$ -\frac{B}{2} \pm z  $$

$$ -\frac{B}{2} \pm  \sqrt{ \left( \frac{B}{2} \right)^2 - C  } $$

Tricks to memorize:

1. Two quantities $B/2$ and $C$. Remember as $B$ is half as good as $A$
   or is the second letter.

2. Besides the $\pm$ sign, all values are negative (could write second
   $B/2$ as negative, wouldn't change result).

3. Square and square roots go together.
